haskell/Optics2/src/Template.hs
@@ -1,0 +1,8 @@
+module  Template
+    (   myFunc
+    )   where
+
+import Control.Lens
+
+myFunc :: IO ()
+myFunc = putStrLn "This is my func"
