lean/exercise_7_10_3.lean
@@ -1,1 +1,29 @@
-TODO
+
+inductive Expr : Type
+| Const : ℕ → Expr
+| Var   : ℕ → Expr
+| Plus  : Expr → Expr → Expr
+| Times : Expr → Expr → Expr
+
+open Expr
+
+def Env : Type := ℕ → ℕ
+
+def eval (env : Env) (e: Expr) : ℕ :=
+  Expr.rec_on e
+    (λ n, n)
+    (λ n, env n)
+    (λ _ _ v1 v2, v1 + v2)
+    (λ _ _ v1 v2, v1 * v2)
+
+def env : Env := λ n, n
+
+
+lemma L1 : eval env (Const 45) = 45 := rfl
+lemma L2 : eval env (Var 34) = 34 := rfl
+lemma L3 : eval env (Plus (Const 5) (Var 6)) = 11 := rfl
+lemma L4 : eval env (Times (Const 5) (Const 6)) = 30 := rfl
+
+
+
+
