coq/cttwc/normalproof.v
@@ -32,3 +32,86 @@ Definition L13 (X Y Z:Prop): (X /\ Y) /\ Z -> X /\ (Y /\ Z) := fun p =>
         | conj x y => conj x (conj y z)
         end
     end. 
+
+Definition L14 (X Y:Prop) : X /\ Y <-> Y /\ X := conj
+    (fun p => match p with conj x y => conj y x end)
+    (fun p => match p with conj y x => conj x y end).
+
+Definition L15 (X Y Z:Prop) : X /\ (Y /\ Z) <-> (X /\ Y) /\ Z := conj
+    (fun p => match p with conj x (conj y z) => conj (conj x y) z end)
+    (fun p => match p with conj (conj x y) z => conj x (conj y z) end).
+
+Definition L16 (X Y Z:Prop) : X /\ (Y \/ Z) <-> X /\ Y \/ X /\ Z := conj
+    (fun p => 
+        match p with conj x yz => 
+            match yz with
+            | or_introl y   => or_introl (conj x y)
+            | or_intror z   => or_intror (conj x z)
+            end
+        end)
+    (fun p =>
+        match p with
+        | or_introl (conj x y)  => conj x (or_introl y)
+        | or_intror (conj x z)  => conj x (or_intror z)
+        end).
+
+Definition L17 (X Y:Prop) : X /\ (X \/ Y) <-> X := conj
+    (fun p => match p with conj x _ => x end)
+    (fun x => conj x (or_introl x)).
+
+
+Definition L18 (X Y:Prop) : X \/ Y <-> Y \/ X := conj
+    (fun p => match p with
+        | or_introl x   => or_intror x
+        | or_intror y   => or_introl y
+        end)
+    (fun p => match p with
+        | or_introl y   => or_intror y
+        | or_intror x   => or_introl x
+        end). 
+
+Definition L19 (X Y Z:Prop) : X \/ (Y \/ Z) <-> (X \/ Y) \/ Z := conj
+    (fun p =>
+        match p with 
+        | or_introl x   => or_introl (or_introl x)
+        | or_intror q   =>
+            match q with
+            | or_introl y   => or_introl (or_intror y)
+            | or_intror z   => or_intror z
+            end
+        end)
+    (fun p =>
+        match p with 
+        | or_introl q =>
+            match q with
+            | or_introl x   => or_introl x
+            | or_intror y   => or_intror (or_introl y)
+            end
+        | or_intror z       => or_intror (or_intror z)
+        end).
+
+Definition L20 (X Y Z:Prop) : X \/ (Y /\ Z) <-> (X \/ Y) /\ (X \/ Z) := conj
+    (fun p => match p with
+        | or_introl x           => conj (or_introl x) (or_introl x)
+        | or_intror (conj y z)  => conj (or_intror y) (or_intror z)
+        end)
+    (fun p => 
+        match p with conj py pz =>
+            match py with
+            | or_introl x   => or_introl x
+            | or_intror y   =>
+                match pz with
+                | or_introl x => or_introl x
+                | or_intror z => or_intror (conj y z)
+                end
+            end
+        end).
+
+Definition L21 (X Y:Prop) : X \/ (X /\ Y) <-> X := conj
+    (fun p  =>
+        match p with
+        | or_introl x           => x
+        | or_intror (conj x y)  => x
+        end)
+    (fun x => or_introl x).
+        
