lean/pattern.lean
@@ -1,0 +1,41 @@
+open nat
+
+def sub1 : ℕ → ℕ
+| zero     := zero
+| (succ x) := x
+
+
+def is_zero : ℕ → Prop
+| zero     := true
+| (succ x) := false
+
+
+example : sub1 0 = 0 := rfl
+example (n : ℕ) : sub1 (succ n) = n := rfl
+
+example : is_zero 0 = true := rfl
+example (n : ℕ) : is_zero (succ n) = false := rfl
+
+
+example : sub1 7 = 6 := rfl
+example (n : ℕ) : ¬ is_zero (n + 3) := begin  simp [is_zero]end
+
+def sub1' : ℕ → ℕ
+| 0 := 0
+| (n+1) := n
+
+universes u v
+variables {α : Type u} {β : Type v}
+
+def swap : α × β → β × α
+| (x,y) := (y,x)
+
+def foo : ℕ × ℕ → ℕ
+| (m,n) := m + n
+
+def bar : option ℕ → ℕ
+| (some n) := n + 1
+| none     := 0
+
+
+
