haskell/Optics2/ChangeLog.md
@@ -1,0 +1,3 @@
+# Changelog for Optics2
+
+## Unreleased changes
